\subsection{Interpolation}\label{subsec:interpolation}
Current manuscript starts from certain interpolation technique shown on base case of cubes, where the key
identity is the tricky rearrangement terms of the sum $\sum_k \Delta k^3$ in~\eqref{eq:rearranged-cubes}.
This rearrangement was done instead of applying Faulhaber's formula on $\Delta n^3 = 1 + 6\sum_{k=1}^{n} k$ which
leads to well-known result involving Binomial theorem:
$(n+1)^3 - n^3 = 1 + 6\sum_{k=1}^{n} k = 1 + 6 \frac{1}{2}(n+n^2) = 1 + 3n^3 + 3n$.
